Adding typing for expressions
Summary:
- adding expression typing: `ok`. Let's find a better name :D
- proof that well-typed expression always evaluate to well-typed values (with
  the same type).

Reviewed By: grievejia

Differential Revision: D18137879

fbshipit-source-id: 2f4d582b8c365472303300a5c96219412170ae12

docs/formal/python_semantic/Eval.v
@@ -107,11 +107,6 @@ Fixpoint eval (now: EState) (expr : Expression.t) : option Value.t :=
             end
     | Expression.Id id => get_state_value now id
     | Expression.None => Some Value.None
-    | Expression.Set_ el =>
-            match eval_list now el with
-            | Some vl => Some (Value.Sequence vl)
-            | None => None
-            end
     | Expression.String s => Some (Value.String s)
     | Expression.Ternary target test alternative =>
             match eval now test with
