docs/formal/python_semantic/Expression.v
@@ -42,7 +42,6 @@ Inductive t: Set :=
   | List: tlist -> t
   | Id: string -> t
   | None: t
-  | Set_: tlist -> t
   | String: string -> t
   | Ternary: forall (target: t) (test: t) (alternative: t), t
   | True_: t
