docs/formal/python_semantic/Semantic.v
@@ -1,0 +1,643 @@
+Require Import List ZArith String.
+Require Pyre.Lvalue.
+Require Pyre.Value.
+Require Pyre.Expression.
+Require Import Pyre.Eval.
+Require Pyre.Statement.
+Require Pyre.Typ.
+Require Import Pyre.Map.
+
+Import Pyre.Value.ListHelpers.
+Import Pyre.Typ.ListHelpers.
+Import Pyre.Expression.ListHelpers.
+
+(** * Typing judgements *)
+
+(** Typing context (Map from identifiers to types) *)
+Definition TContext := RawState0 Typ.t.
+
+Definition get_context_type (ctx: TContext) (k: string) : option Typ.t :=
+    get0 _ ctx k.
+
+Section TypingExpression.
+
+Import Pyre.Expression.
+
+(** Typing judgement for expressions *)
+Inductive ok : TContext -> Expression.t -> Typ.t -> Prop :=
+  | typFalse: forall ctx, ok ctx False_ Typ.Boolean
+  | typTrue: forall ctx, ok ctx True_ Typ.Boolean
+  | typInteger: forall ctx z, ok ctx (Integer z) Typ.Integer
+  | typString: forall ctx str, ok ctx (String str) Typ.String
+  | typNone: forall  ctx,  ok ctx None Typ.None
+  | tyBop: forall ctx b0 b1 op,
+          ok ctx b0 Typ.Boolean ->
+          ok ctx b1 Typ.Boolean ->
+          ok ctx (BooleanOperator b0 op b1) Typ.Boolean
+  | tyCmp: forall ctx e0 e1 op,
+          ok ctx e0 Typ.Integer ->
+          ok ctx e1 Typ.Integer ->
+          ok ctx (ComparisonOperator e0 op e1) Typ.Boolean
+  | TyList: forall ctx (l: Expression.tlist) ty,
+          ok_list ctx l ty -> 
+          ok ctx (List l) (Typ.List ty)
+  | TyTuple: forall ctx (l: Expression.tlist) lty,
+          ok_tuple ctx l lty ->
+          ok ctx (Tuple l) (Typ.Tuple lty)
+  | TyNot: forall ctx expr,
+          ok ctx expr Typ.Boolean ->
+          ok ctx (UnaryOperator Not expr) Typ.Boolean
+  | TyUnary: forall ctx expr op,
+         op <> Not -> 
+         ok ctx expr Typ.Integer ->
+         ok ctx (UnaryOperator op expr) Typ.Integer
+  | TyTernary : forall ctx target test alternative typ,
+          ok ctx target typ ->
+          ok ctx alternative typ ->
+          ok ctx test Typ.Boolean ->
+          ok ctx (Ternary target test alternative) typ
+  | TyId: forall ctx id T,
+          get_context_type ctx id = Some T ->
+          ok  ctx (Id id) T
+with ok_list: TContext -> Expression.tlist -> Typ.t -> Prop :=
+  | tyListNil : forall ctx typ, ok_list ctx Nil typ
+  | tyListCons : forall ctx hd tl typ,
+          ok ctx hd typ ->
+          ok_list ctx tl typ ->
+          ok_list ctx (Cons hd tl) typ
+with ok_tuple : TContext -> Expression.tlist -> Typ.tlist -> Prop :=
+  | tyTupleSingl : forall ctx expr typ,
+          ok ctx expr typ ->
+          ok_tuple ctx (Cons expr Nil) (Typ.Cons typ Typ.Nil)
+  | tyTupleCons : forall ctx expr le typ lt,
+          ok ctx expr typ ->
+          ok_tuple ctx le lt ->
+          ok_tuple ctx (Cons expr le) (Typ.Cons typ lt)
+.
+
+(* begin hide *)
+Scheme ok_ind' := Induction for ok Sort Prop
+  with ok_list_ind' := Induction for ok_list Sort Prop
+  with ok_tuple_ind' := Induction for ok_tuple Sort Prop.
+
+Combined Scheme ok_induc from ok_ind', ok_list_ind', ok_tuple_ind'.
+
+Lemma ok_tuple_len: forall ctx le lt,
+    ok_tuple ctx le lt -> List.length le = List.length lt.
+Proof.
+intro ctx.
+induction 1; simpl in *; now intuition.
+Qed.
+
+Lemma ok_tuple_len_pos : forall ctx le lt,
+    ok_tuple ctx le lt -> List.length le > 0.
+Proof.
+intro ctx.
+induction 1; simpl in *; now intuition.
+Qed.
+
+Lemma ok_list_spec: forall ctx l typ,
+    ok_list ctx l typ -> Forall (fun expr => ok ctx expr typ) l.
+Proof.
+induction 1 as [ ctx typ | ctx hd tl typ h0 h1 hi ];
+    [ now apply Forall_nil | ].
+now apply Forall_cons.
+Qed.
+
+Lemma ok_list_forall: forall ctx (l: Expression.tlist) typ,
+    Forall (fun expr => ok ctx expr typ) l -> ok_list ctx l typ.
+Proof.
+intro ctx.
+induction l as [ | hd tl hi]; intros typ h; inversion h; subst; clear h.
+- now constructor.
+- apply hi in H2.
+  now constructor.
+Qed.
+
+Lemma ok_tuple_spec: forall ctx l lt, ok_tuple ctx l lt ->
+    List.length l > 0 /\
+    List.length l = List.length lt /\
+    Forall (fun et => ok ctx (fst et) (snd et)) (List.combine l lt).
+Proof.
+induction 1 as [ctx expr typ h | ctx expr typ es et h hs hi ].
+- intuition.
+  now apply Forall_cons.
+- now simpl; intuition.
+Qed.
+
+Lemma ok_tuple_forall: forall ctx (l: Expression.tlist) (lt: Typ.tlist),
+    List.length l > 0 ->
+    List.length l = List.length lt ->
+    Forall (fun et => ok ctx (fst et) (snd et)) (List.combine l lt) ->
+    ok_tuple ctx l lt.
+Proof.
+induction l as [ | hd tl hi];
+       intros lt hp hl h; inversion h; subst; clear h; simpl in *.
+- now idtac.
+- destruct lt as [ | typ typs]; [now idtac | ]. 
+  simpl in H0.
+  discriminate H0.
+- destruct x as [v' t']; simpl in *.
+  destruct lt as [ | typ typs]; [now idtac | ]. 
+  injection hl; clear hl; intro hl.
+  simpl in H; injection H; clear H; intros heq0 heq1; subst.
+  (* special case for list of size 1 *)
+  case_eq tl.
+  + intros ? h; subst.
+    simpl in hl.
+    destruct typs as [ | ]; [ | now idtac].
+    now constructor.
+  + intros ? ? htl ?; subst.
+    constructor; [ now idtac | ].
+    now apply hi; simpl; intuition.
+Qed.
+
+Lemma ok_tuple_forall2: forall ctx (l: Expression.tlist) (lt: Typ.tlist),
+    List.length lt > 0 ->
+    List.length l = List.length lt ->
+    Forall (fun et => ok ctx (fst et) (snd et)) (List.combine l lt) ->
+    ok_tuple ctx l lt. 
+Proof.
+intros ctx l lt h heq hf.
+now apply ok_tuple_forall; intuition.
+Qed.
+(* end hide *)
+
+End TypingExpression.
+
+Hint Constructors ok ok_list ok_tuple : core.
+
+Section TypingValue.
+
+Import Value.
+
+(** Typing judgement for values *)
+Inductive okv : Value.t -> Typ.t -> Prop :=
+  | TyVBoolean: forall b, okv (Boolean b) Typ.Boolean
+  | TyVInteger: forall i, okv (Integer i) Typ.Integer
+  | TyVString: forall str, okv (String str) Typ.String
+  | TyVList: forall (l: Value.tlist) T,
+          okv_list l T ->
+          okv (Sequence l) (Typ.List T)
+  | TyVTuple: forall (l: Value.tlist) (lt: Typ.tlist),
+          okv_tuple l lt ->
+          okv (Sequence l) (Typ.Tuple lt)
+  | TyNone: okv Value.None Typ.None
+with okv_list: Value.tlist -> Typ.t -> Prop :=
+  | TyVNil: forall typ, okv_list Nil typ
+  | TyVCons: forall hd tl typ,
+          okv hd typ ->
+          okv_list tl typ ->
+          okv_list (Cons hd tl) typ
+with okv_tuple: Value.tlist -> Typ.tlist -> Prop :=
+  | TyVSingle: forall expr typ,
+          okv expr typ ->
+          okv_tuple (Cons expr Nil) (Typ.Cons typ Typ.Nil)
+  | TyVTuples: forall expr typ es typs,
+          okv expr typ ->
+          okv_tuple es typs ->
+          okv_tuple (Cons expr es) (Typ.Cons typ typs)
+.
+
+(* begin hide *)
+Lemma okv_list_spec: forall lv typ, okv_list lv typ ->
+    Forall (fun v => okv v typ) lv.
+Proof.
+induction 1 as [ | hd tl typ h0 h1 hi ]; [ now apply Forall_nil | ].
+now apply Forall_cons.
+Qed.
+
+Lemma okv_list_forall: forall (lv: Value.tlist) typ,
+    Forall (fun v => okv v typ) lv -> okv_list lv typ.
+Proof.
+induction lv as [ | hd tl hi]; intros typ h; inversion h; subst; clear h.
+- now constructor.
+- apply hi in H2.
+  now constructor.
+Qed.
+
+Lemma okv_tuple_spec: forall lv lt, okv_tuple lv lt ->
+    List.length lv > 0 /\
+    List.length lv = List.length lt /\
+    Forall (fun vt => okv (fst vt) (snd vt)) (List.combine lv lt).
+Proof.
+induction 1 as [ expr typ h | expr typ es et h hs hi ].
+- intuition.
+  now apply Forall_cons.
+- now simpl; intuition.
+Qed.
+
+Lemma okv_tuple_forall: forall (lv: Value.tlist) (lt: Typ.tlist),
+    List.length lv > 0 ->
+    List.length lv = List.length lt ->
+    Forall (fun vt => okv (fst vt) (snd vt)) (List.combine lv lt) ->
+    okv_tuple lv lt.
+Proof.
+induction lv as [ | hd tl hi];
+       intros lt hp hl h; inversion h; subst; clear h; simpl in *.
+- now idtac.
+- destruct lt as [ | typ typs]; [now idtac | ]. 
+  simpl in H0.
+  discriminate H0.
+- destruct x as [v' t']; simpl in *.
+  destruct lt as [ | typ typs]; [now idtac | ]. 
+  injection hl; clear hl; intro hl.
+  simpl in H; injection H; clear H; intros heq0 heq1; subst.
+  (* special case for list of size 1 *)
+  case_eq tl.
+  + intros ? h; subst.
+    simpl in hl.
+    destruct typs as [ | ]; [ | now idtac].
+    now constructor.
+  + intros ? ? htl ?; subst.
+    constructor; [ now idtac | ].
+    now apply hi; simpl; intuition.
+Qed.
+
+Lemma okv_tuple_forall2: forall (lv: Value.tlist) (lt: Typ.tlist),
+    List.length lt > 0 ->
+    List.length lv = List.length lt ->
+    Forall (fun vt => okv (fst vt) (snd vt)) (List.combine lv lt) ->
+    okv_tuple lv lt.
+Proof.
+intros lv lt h heq hf.
+now apply okv_tuple_forall; intuition.
+Qed.
+(* end hide *)
+
+End TypingValue.
+
+Hint Constructors okv okv_list okv_tuple : core.
+
+(** Well-formed <<EState>> w.r.t. some <<TContext>>:
+    for any typed variable in the context, there must be a value of the
+    right type associated to in the the state. *)
+Definition well_formed_estate (s : EState) (ctx: TContext) : Prop :=
+    (forall k T, get0 _ ctx k = Some T ->
+     exists v, get0 _ s k = Some v /\ okv v T)
+.
+
+(* begin hide *)
+Lemma well_formed_estate_get: forall s ctx, well_formed_estate s ctx ->
+    forall k T, get_context_type ctx k = Some T -> exists v,
+    get_state_value s k = Some v /\ okv v T.
+Proof.
+intros s ctx hwf k T.
+now apply hwf.
+Qed.
+
+Lemma ty_bool_int : forall ctx expr typ, ok ctx expr typ ->
+    forall s, well_formed_estate s ctx ->
+    (typ = Typ.Boolean -> exists b, eval s expr = Some (Value.Boolean b)) /\
+    (typ = Typ.Integer -> exists z, eval s expr = Some (Value.Integer z)).
+Proof.
+induction 1 as [
+    | ctx
+    | ctx z
+    | ctx str
+    | ctx
+    | ctx left right op hl hil hr hir
+    | ctx left right op hl hil hr hir
+    | ctx l typ hl
+    | ctx l typs hl
+    | ctx expr he hie
+    | ctx expr op hop he hie
+    | ctx target test alterntaive typ htarget hitarget
+            halt hialt htest hitest
+    | ctx id T h
+]; intros s hwf; subst; split; intro heq; subst;
+   try discriminate; simpl in *.
++ now exists false.
++ now exists true.
++ now exists z.
++ destruct (hil s hwf) as [h0 _].
+  destruct (hir s hwf) as [h1 _].
+  destruct (h0 refl_equal) as [x0 hx0].
+  destruct (h1 refl_equal) as [x1 hx1].
+  rewrite hx0, hx1.
+  now exists (evaluate_boolean_operator x0 op x1).
++ destruct (hil s hwf) as [_ h0].
+  destruct (hir s hwf) as [_ h1].
+  destruct (h0 refl_equal) as [x0 hx0].
+  destruct (h1 refl_equal) as [x1 hx1].
+  rewrite hx0, hx1.
+  now exists (evaluate_comparison_operator (Value.Integer x0) op (Value.Integer x1)).
++ destruct (hie s hwf) as [h0 _]. 
+  destruct (h0 refl_equal) as [ x0 hx0 ].
+  rewrite hx0.
+  now exists (negb x0).
++ destruct (hie s hwf) as [_ h0].
+  destruct (h0 refl_equal) as [ x0 hx0 ].
+  rewrite hx0; simpl.
+  rewrite evaluate_unary_int_operator; destruct op; try (now elim hop).
+  * now exists (-x0 -1)%Z.
+  * now exists ( - x0 )%Z.
+  * now exists x0.
++ destruct (hitarget s hwf) as [h0 _].
+  destruct (hialt s hwf) as [h1 _].
+  destruct (hitest s hwf) as [h2 _].
+  destruct (h0 refl_equal) as [x0 hx0].
+  destruct (h1 refl_equal) as [x1 hx1].
+  destruct (h2 refl_equal) as [x2 hx2].
+  rewrite hx2; destruct x2. 
+  * rewrite hx0.
+    now exists x0.
+  * rewrite hx1.
+    now exists x1.
++ destruct (hitarget s hwf) as [_ h0].
+  destruct (hialt s hwf) as [_ h1].
+  destruct (hitest s hwf) as [h2 _].
+  destruct (h0 refl_equal) as [x0 hx0].
+  destruct (h1 refl_equal) as [x1 hx1].
+  destruct (h2 refl_equal) as [x2 hx2].
+  rewrite hx2; destruct x2. 
+  * rewrite hx0.
+    now exists x0.
+  * rewrite hx1.
+    now exists x1.
++ apply well_formed_estate_get with (s := s) in h; [ | now idtac ].
+  destruct h as [ v [-> hv]].
+  inversion hv; subst; clear hv.
+  now exists b.
++ apply well_formed_estate_get with (s := s) in h; [ | now idtac ].
+  destruct h as [ v [-> hv]].
+  inversion hv; subst; clear hv.
+  now exists i.
+Qed.
+(* end hide *)
+
+(** Every expression typed as <<Typ.Boolean>> must  be an actual <<bool>> *)
+Lemma ty_bool : forall ctx expr, ok ctx expr Typ.Boolean ->
+    forall s, well_formed_estate s ctx ->
+    exists b, eval s expr = Some (Value.Boolean b).
+Proof.
+intros ctx expr h s hwf; eapply ty_bool_int in h as [ h0 _].
+- now apply h0.
+- now apply hwf.
+Qed.
+
+(** Every expression typed as <<Typ.Integer>> must  be an actual <<Z>> *)
+Lemma ty_int : forall ctx expr, ok ctx expr Typ.Integer ->
+    forall s, well_formed_estate s ctx ->
+    exists z, eval s expr = Some (Value.Integer z).
+Proof.
+intros ctx expr h s hwf; eapply ty_bool_int in h as [ _ h0].
+- now apply h0.
+- now apply hwf.
+Qed.
+
+(* begin hide *)
+Lemma ty_string_ : forall ctx expr typ, ok ctx expr typ -> 
+    typ = Typ.String -> forall s, well_formed_estate s ctx ->
+    exists str, eval s expr = Some (Value.String str).
+Proof.
+induction 1 as [
+    | ctx
+    | ctx z
+    | ctx str
+    | ctx
+    | ctx left right op hl hil hr hir
+    | ctx left right op hl hil hr hir
+    | ctx l typ hl
+    | ctx l typs hl
+    | ctx expr he hie
+    | ctx expr op hop he hie
+    | ctx target test alterntaive typ htarget hitarget
+            halt hialt htest hitest
+    | ctx id T h
+] ; intros heq s hwf; subst; try discriminate; simpl in *.
+- now exists str.
+- apply ty_bool with (s := s) in htest as [ b hb ];[ | now idtac ].
+  rewrite hb.
+  destruct (hitarget refl_equal s hwf) as [s1 hs1].
+  destruct (hialt refl_equal s hwf) as [s2 hs2].
+  rewrite hs1, hs2.
+  destruct b.
+  + now exists s1.
+  + now exists s2.
+- apply well_formed_estate_get with (s := s) in h; [ | now idtac].
+  destruct h as [v [-> hv]].
+  inversion hv; subst; clear hv.
+  now exists str.
+Qed.
+(* end hide *)
+
+(** Every expression typed as <<Typ.String>> must  be an actual <<string>> *)
+Lemma ty_string : forall ctx expr, ok ctx expr Typ.String ->
+    forall s, well_formed_estate s ctx ->
+    exists str, eval s expr = Some (Value.String str).
+Proof.
+intros ctx expr h s hwf.
+now apply ty_string_ with (ctx := ctx) (s := s) in h.
+Qed.
+
+(* begin hide *)
+Lemma ty_none_: forall ctx expr typ, ok ctx expr typ ->
+    typ = Typ.None -> forall s, well_formed_estate s ctx ->
+    eval s expr = Some Value.None.
+Proof.
+induction 1 as [
+    | ctx
+    | ctx z
+    | ctx str
+    | ctx
+    | ctx left right op hl hil hr hir
+    | ctx left right op hl hil hr hir
+    | ctx l typ hl
+    | ctx l typs hl
+    | ctx expr he hie
+    | ctx expr op hop he hie
+    | ctx target test alterntaive typ htarget hitarget
+            halt hialt htest hitest
+    | ctx id T h
+] ; intros heq s hwf; subst; try discriminate; simpl in *.
+- reflexivity.
+- apply ty_bool with (s := s) in htest as [ b hb ];[ | now idtac ].
+  rewrite hb.
+  rewrite (hitarget refl_equal s hwf).
+  rewrite (hialt refl_equal s hwf).
+  now destruct b.
+- apply well_formed_estate_get with (s := s) in h; [ | now idtac].
+  destruct h as [v [-> hv]].
+  inversion hv; subst; clear hv.
+  reflexivity.
+Qed.
+(* end hide *)
+
+(** Every expression typed as <<Typ.None>>  must be <<None>> *)
+Lemma ty_none: forall ctx expr, ok ctx expr Typ.None ->
+    forall s, well_formed_estate s ctx -> eval s expr = Some Value.None.
+Proof.
+intros  ctx expr h s hwf.
+now apply ty_none_ with (ctx := ctx) (s := s) in h.
+Qed.
+
+Definition is_sequence (typ : Typ.t) : option Typ.t :=
+    match typ with
+    | Typ.List T => Some T
+    | _ => None
+    end.
+
+Definition is_tuple (typ : Typ.t) : list Typ.t :=
+    match typ with
+    | Typ.Tuple l => l
+    | _ => nil
+end.
+
+(** * Type soundness
+
+    Proof that a correctly typed expression always evaluate to a value,
+    and this value has the same type as the input expression.
+*)
+
+Lemma eval_ok_ :
+    (forall ctx expr typ, ok ctx expr typ ->
+        forall s, well_formed_estate s ctx ->
+        exists v, eval s expr = Some v /\  okv v typ) /\
+    (forall ctx le typ, ok_list ctx le typ ->
+        forall s, well_formed_estate s ctx ->
+        exists lv, eval_list s le = Some lv /\
+        okv_list lv typ) /\
+    (forall ctx le lt, ok_tuple ctx le lt ->
+        forall s, well_formed_estate s ctx ->
+        exists lv, eval_list s le = Some lv /\ okv_tuple lv lt).
+Proof.
+apply ok_induc.
+(* ok *)
+- intros ctx s hwf; subst; exists (Value.Boolean false); now split.
+- intros ctx s hwf; subst; exists (Value.Boolean true); now split.
+- intros ctx z s hwf; subst; exists (Value.Integer z); now split.
+- intros ctx str s hwf; subst; exists (Value.String str); now split.
+- intros ctx s hwf; subst; exists Value.None; now split.
+- intros ctx b0 b1 op h0 ? h1 ? s hwf; simpl; subst.
+  apply ty_bool with (s := s) in h0; [ | now idtac].
+  destruct h0 as [vb0 ->].
+  apply ty_bool with (s := s) in h1; [ | now idtac ].
+  destruct h1 as [vb1 ->].
+  now eexists; split; [ reflexivity | idtac].
+- intros ctx e0 e1 op h0 ? h1 ? s hwf; simpl; subst.
+  apply ty_int with (s := s) in h0; [ | now idtac ].
+  destruct h0 as [v0 ->].
+  apply ty_int with (s := s) in h1; [ | now idtac ].
+  destruct h1 as [v1 ->].
+  now eexists; split; [ reflexivity | idtac].
+- intros ctx l ty h hi s hwf; simpl.
+  destruct (hi _ hwf) as  [vl [-> h0]].
+  now eexists; split; [reflexivity  | constructor ].
+- intros ctx l ty h hi s hwf; simpl.
+  destruct (hi _ hwf) as  [vl [-> h0]].
+  now eexists; split; [reflexivity  | constructor ].
+- intros ctx expr h hi s hwf; simpl.
+  apply ty_bool with (s := s) in h as [v ->]; [ | now idtac ].
+  now eexists; split; [reflexivity | ].
+- intros ctx expr op hop h hi s hwf; simpl.
+  apply ty_int with (s := s) in h as [v ->]; [ | now idtac ].
+  rewrite evaluate_unary_int_operator.
+  destruct op; try (now elim hop); now eexists; split; [reflexivity | ].
+- intros ctx target test alt typ htarget hitarget halt hialt htest hitest
+    s hwf; simpl.
+  apply ty_bool with (s := s) in htest as [b ->]; [ | now idtac ].
+  destruct (hitarget _ hwf) as [vt [-> hvt]].
+  destruct (hialt _ hwf) as [va [-> hva]].
+  now destruct b; eexists; split; [ reflexivity | | reflexivity | ].
+- intros ctx id typ hg s hwf; simpl.
+  now apply well_formed_estate_get with (ctx := ctx); [ now apply hwf | ].
+(* ok_list *)
+- intros ctx typ s hwf; simpl.
+  now exists Value.Nil; intuition.
+- intros ctx hd tl typ h0 hi0 h1 hi1 s hwf; simpl.
+  destruct (hi0 _ hwf) as [vhd [-> hv]].
+  destruct (hi1 _ hwf) as [vtl [-> ht]].
+  now exists (Value.Cons vhd vtl); intuition.
+(* ok_tuple *)
+- intros ctx expr typ h hi s hwf; simpl.
+  destruct (hi _ hwf) as [v [-> ?]].
+  now  exists (Value.Cons v Value.Nil); intuition.
+- intros ctx expr el typ tl h0 hi0 h1 hi1 s hwf; simpl.
+  destruct (hi0 _ hwf) as [vhd [-> ?]].
+  destruct (hi1 _ hwf) as [vtl [-> ?]].
+  now exists (Value.Cons vhd vtl); intuition.
+Qed.
+
+Lemma eval_ok: forall ctx expr typ, ok ctx expr typ ->
+    forall s, well_formed_estate s ctx ->
+    exists v, eval s expr = Some v /\ okv v typ.
+Proof.
+intros.
+now eapply eval_ok_; eauto.
+Qed.
+
+Lemma eval_list_ok: forall ctx le typ, ok_list ctx le typ ->
+    forall s, well_formed_estate s ctx ->
+    exists lv, eval_list s le = Some lv /\ okv_list lv typ.
+Proof.
+intros.
+now eapply eval_ok_; eauto.
+Qed.
+
+Lemma eval_tuple_ok: forall ctx le lt, ok_tuple ctx le lt ->
+    forall s, well_formed_estate s ctx ->
+    exists lv, eval_list s le = Some lv /\ okv_tuple lv lt.
+Proof.
+intros.
+now eapply eval_ok_; eauto.
+Qed.
+
+Lemma ok_sequence : forall ctx expr T, ok ctx expr T ->
+    forall T', is_sequence T = Some T' ->
+    forall s, well_formed_estate s ctx ->
+    exists lv, eval s expr = Some (Value.Sequence lv).
+Proof.
+induction 1 as [
+    | ctx
+    | ctx z
+    | ctx str
+    | ctx
+    | ctx left right op hl hr
+    | ctx left right op hl hr
+    | ctx l typ hl
+    | ctx l typs hl
+    | ctx expr he
+    | ctx expr op hop he
+    | ctx target test alterntaive typ htarget hit halt hia htest hitest
+    | ctx id T h
+]; intros T' hT s hwf; simpl; subst;
+  try (unfold is_sequence in hT; simpl in hT; discriminate).
+- apply eval_list_ok with (s := s) in hl as [lv [-> ?]]; [ | now idtac ].
+  now exists lv.
+- destruct (hit T' hT s hwf) as [l1 ->].
+  destruct (hia T' hT s hwf) as [l2 ->].
+  apply ty_bool with (s := s) in htest as [b ->]; [ | now idtac ].
+  now destruct b; eexists; reflexivity.
+- apply well_formed_estate_get with (s := s) in h as [v [-> h1]];
+    [ | now idtac ].
+  inversion h1; subst; clear h1; try discriminate; now eexists; reflexivity.
+Qed.
+
+Lemma ty_list: forall ctx expr T, ok ctx expr (Typ.List T) ->
+    forall s, well_formed_estate s ctx ->
+    exists lv, eval s expr = Some (Value.Sequence lv) /\
+               okv (Value.Sequence lv) (Typ.List T).
+Proof.
+intros ctx expr T hok s hwf.
+apply eval_ok with (s := s) in hok; [ | now idtac].
+destruct hok as [v [-> hv]].
+inversion hv; subst; clear hv.
+exists l; split; [ now idtac | ].
+now constructor.
+Qed.
+
+(* begin hide *)
+Lemma well_formed_estate_set: forall s ctx,
+  well_formed_estate s ctx ->
+  forall id v T, okv v T ->
+  well_formed_estate (set0 _ s id v) (set0 _ ctx id T).
+Proof.
+intros s ctx hwf id v T hok.
+intros k S; unfold set, set0, get0; simpl.
+rewrite !get_set_map.
+destruct String.eqb.
+- intro h; injection h; clear h; intro; subst.
+  now exists v.
+- now apply hwf.
+Qed.
